some explanation comments

sec/Semantics.thy
@@ -95,7 +95,7 @@ lemma twoPredLiftI[intro]:
 definition sec_agree
   :: \<open>('a \<Rightarrow> 'v) \<Rightarrow> 'a \<times> 'a \<Rightarrow> bool\<close> (\<open>\<bbbA>\<close>)
   where
-    \<open>\<bbbA> vf \<equiv> (\<lambda>(ab,ab'). vf ab = vf ab')\<close>
+    \<open>\<bbbA> vf \<equiv> (\<lambda>(x,y). vf x = vf y)\<close>
 
 lemma conj_agree_iff:
   \<open>\<bbbA> v1 \<sqinter> \<bbbA> v2 = \<bbbA> (\<lambda>x. (v1 x, v2 x))\<close>
@@ -465,6 +465,93 @@ proof -
     done
 qed
 
+(* 
+Let c be a simple program that operates on a single state and 
+let \<oo> be  a function describing the observations the attacker can make on a given state,
+the function (liftC \<oo> c) turns the program c into one that operates on a pair of states and that crashes
+when run on states that are distingishable through  \<oo>. This in turn, which can be  used for info flow reasoning.
+
+
+
+the safe judgement provides the same amount of information as a programming language semantics that 
+is a tree T of all possible executions that can happen, as well as a proof that if the precondition and 
+the relies, then for all possible executions in the tree
+   (1) they don't fail and
+   (2) the obey the guarantees and the postcondition
+   (3) the frame condition is preserved
+
+
+define function f ( c, n, p, r) = trees T
+
+prove
+theorems 
+safe_imp_no_crash:"safe  c, n, p, r, q,g \<longrightarrow> 
+  (1) the program f ( c, n, p, r) does not crash,
+  (2) the program  obey the guarantees and the postcondition
+  (3) the frame condition is preserved
+
+
+definition noninterference is: given a pair of states s1 and s2, indistinguishable by \<oo>,
+no execution of the program on s1 and s2 respectively, are pair-wise indistinguishable by \<oo> throughout execution and 
+the program executions match/allign.
+
+
+-------
+
+definition noninterference is: given a pair of states, indistinguishable by \<oo>,
+no execution of the program c (lifted to pairs of states) reaches a pair of states distinguishable by \<oo>.
+
+definition noninterference on (liftC \<oo> c) is also a property s.t.
+given a pair of states that are indistinguishable through \<oo>, of the program  (liftC \<oo> c) doesn't fail 
+then all pairs of states throughout the 
+execution of liftC \<oo> c are indistinguishable.
+
+the noninterference judgement on (liftC \<oo> c) provides the same amount of information as a programming language semantics that 
+is a tree T of all possible executions that can happen on pairs of states, as well as a proof that if the precondition and 
+the relies hold and the precondition respects  \<oo>, then for all possible executions in the tree
+   if the program doesn't fail 
+    the indistinguishability predicate is preserved
+
+
+(do we also want the frame condition to be preserved)
+
+question
+is there anything other than no-crash that is needed to prove non-interference and (e.g. there is no non-determinism), potentially?
+
+if not,
+
+prove 
+theorem noninterference: 
+
+
+If we can prove this, we are done (with the security paper).
+
+question 
+can we change liftC to not crash
+then instead prove
+>how can we generalise the lifting function liftC and instead of crashing 
+ instantiate the guarantee in a way that enforces non-interference/indistinguishability?
+
+then pro
+
+If the preconditions are indistinguishable using \<oo>, and the lifted program  (liftC \<oo> c)  is safe,
+and the preconditinos are indistinguishable using \<oo>.
+
+If the preconditions are indistinguishable using \<oo>, and the lifted program  (liftC \<oo> c)  is safe,
+and the preconditinos are indistinguishable using \<oo>.
+
+
+
+
+
+properties (p, r) do not crash
+these executions will 
+and you can also extract a tree semantics that only contains 
+split to two pieces, one is all possible executions, and the other is 
+function to filter safe executions out of safe judgement
+if there is no crashing anywhere 
+
+define noninterference directly on liftC o C
 
 lemma exact_security:
   fixes hl1 hl2 :: \<open>'l :: pre_perm_alg\<close>
@@ -473,8 +560,34 @@ lemma exact_security:
     and p q :: \<open>'l \<times> 's \<Rightarrow> bool\<close>
     and r g :: \<open>'s \<Rightarrow> 's \<Rightarrow> bool\<close>
   shows
-  \<open>trace_step_align t1 t2 \<Longrightarrow>
-    safe
+  \<open>safe
+      (max (alength t1) (alength t2))
+      (liftC \<oo> c)
+      (Inl (exch4 (fst (ahd t1), fst (ahd t2))))
+      (liftR r) (liftR g)
+      (liftP q \<circ> exch4)
+      (liftP S \<circ> exch4) (liftP F \<circ> exch4) \<Longrightarrow>f ( c, n, p, r) 
+no_crashing \<and> indistinguishable everywhere through initial_s p c  \<oo>  >
+*)
+
+
+(*
+lemma exact security
+<no_crashing \<Longrightarrow>
+    t1 \<in> trsem p q r g S F c \<Longrightarrow>
+    t2 \<in> trsem p q r g S F c \<Longrightarrow>
+    trace_step_align t1 t2 \<Longrightarrow>
+    \<lblot> p \<rblot> \<le> \<bbbA> \<oo> \<Longrightarrow>
+    trace_agree (apfst \<oo>) t1 t2\<close>
+*)
+lemma exact_security:
+  fixes hl1 hl2 :: \<open>'l :: pre_perm_alg\<close>
+    and hs1 hs2 :: 's
+    and c :: \<open>('l \<times> 's, unit) comm\<close>
+    and p q :: \<open>'l \<times> 's \<Rightarrow> bool\<close>
+    and r g :: \<open>'s \<Rightarrow> 's \<Rightarrow> bool\<close>
+  shows
+  \<open>safe
       (max (alength t1) (alength t2))
       (liftC \<oo> c)
       (Inl (exch4 (fst (ahd t1), fst (ahd t2))))
@@ -483,6 +596,7 @@ lemma exact_security:
       (liftP S \<circ> exch4) (liftP F \<circ> exch4) \<Longrightarrow>
     t1 \<in> trsem p q r g S F c \<Longrightarrow>
     t2 \<in> trsem p q r g S F c \<Longrightarrow>
+    trace_step_align t1 t2 \<Longrightarrow>
     \<lblot> p \<rblot> \<le> \<bbbA> \<oo> \<Longrightarrow>
     trace_agree (apfst \<oo>) t1 t2\<close>
 proof (induct rule: trace_step_align.inducts)
@@ -503,11 +617,11 @@ next
     apply clarsimp
     apply (clarsimp simp add: safe_suc_iff)
     apply (rule tragree_step_left_tau)
-    sledgehammer
-    by (smt (verit) ahd.simps(2) alength_simps(2) fst_conv max.cobounded2 max.orderE max_def_raw mem_Collect_eq not_less_eq_eq safe_step_SucD step_left_tau.hyps(2) step_left_tau.prems(1) step_left_tau.prems(3) step_left_tau.prems(4) trsem_def)
-    sorry
-    apply (metis (no_types, lifting) le_Suc_eq max_def)
-    done
+
+    by (smt (verit) ahd.simps(2) alength_simps(2) fst_conv max.cobounded2 max.orderE 
+                    max_def_raw mem_Collect_eq not_less_eq_eq safe_step_SucD step_left_tau.hyps(2) 
+                    step_left_tau.prems(1) step_left_tau.prems(3) step_left_tau.prems(4) trsem_def)
+
 next
   case (step_right_tau t1 t2 s2)
   then show ?case
